lazy_list/spec/contains.v
@@ -17,42 +17,56 @@ Module ContainsSpec (Params: LAZY_LIST_PARAMS).
   Section Proofs.
     Context `{!heapGS Σ, !gset_list_unionGS Σ, !lockG Σ}.
     
-    Theorem find_spec (key: Z) (head curr: node_rep) (S: gset node_rep) (Γ: lazy_gname) :
+    Theorem find_spec (key: Z) (head curr: node_rep) (Skeys: gset Z) (Γ: lazy_gname) :
       {{{ 
         inv lazyN (lazy_list_inv head Γ)
         ∗
-        own (s_frac Γ) (◯F S)
+        own (s_frac Γ) (◯F Skeys)
         ∗
-        ⌜ curr = head ∨ curr ∈ S ⌝
+        (⌜ curr = head ⌝ ∨ own (s_auth Γ) (◯ {[curr]}))
         ∗
         ⌜ node_key curr < key < INT_MAX ⌝
       }}}
       find (rep_to_node curr) #key
       {{{ pred succ, RET SOMEV ((rep_to_node pred), (rep_to_node succ));
-        own (s_frac Γ) (◯F S)
+        own (s_frac Γ) (◯F Skeys)
         ∗
-        ⌜ key ∈ map node_key (elements S) ↔ node_key succ = key ⌝
+        ⌜ key ∈ Skeys ↔ node_key succ = key ⌝
       }}}.
     Proof.
-      iIntros (Φ) "(#Hinv & Hown_frag & Hcurr_range & Hrange) HΦ".
-      iRevert (curr) "Hown_frag Hcurr_range Hrange HΦ".
+      iIntros (Φ) "(#Hinv & Hown_frag & Hown_curr & Hrange) HΦ".
+      iRevert (curr) "Hown_frag Hown_curr Hrange HΦ".
       iLöb as "IH".
-      iIntros (curr) "Hown_frag %Hcurr_range %Hrange HΦ".
+      iIntros (curr) "Hown_frag #Hown_curr %Hrange HΦ".
       wp_lam. wp_let. wp_lam. wp_pures.
 
       destruct (node_next curr) as [l|] eqn:Hcurr_next; wp_pures.
       + wp_bind (Load _). 
-        iInv lazyN as (S' Skeys L) "(>%Hperm & >%Hsort & >%Hequiv & >Hown_auth & >Hown_frac & >Hown_keys & Hlist)" "Hclose".
+        iInv lazyN as (S ? L) "(>%Hperm & >%Hsort & >%Hequiv & >Hown_auth & >Hown_frac & >Hown_keys & Hlist)" "Hclose".
         iDestruct (own_valid_2 with "Hown_frac Hown_frag") 
           as %->%frac_auth_agree_L.
 
+        iAssert ((⌜ curr = head ∨ In curr L ⌝)%I) with "[Hown_auth Hown_curr]" as %Hcurr_range.
+        {
+         iDestruct "Hown_curr" as "[Heq|Hown]"; first by iLeft.
+         iDestruct (own_valid_2 with "Hown_auth Hown") 
+          as %[Hvalid%gset_included]%auth_both_valid_discrete.
+         iPureIntro; right.
+         rewrite -elem_of_list_In Hperm elem_of_elements.
+         set_solver.
+        }
+
         edestruct (in_split curr ([head] ++ L)) 
           as (Ls&Lf&Hcurr).
-        { destruct Hcurr_range; first by left.
-          by right; rewrite -elem_of_list_In Hperm elem_of_elements. }
+        { rewrite in_inv //. }
   
         edestruct (node_rep_split_join Lf curr key) 
-          as (pred&succ&L1&L2&?&Hsplit_join); auto.
+          as (pred&succ&L1&L2&?&?&Hsplit_join); auto.
+        {
+          rewrite -app_ass Hcurr app_ass in Hsort.
+          apply node_rep_sorted_app in Hsort.
+          simpl in *. by destruct Hsort as [_ ?].
+        }
   
         feed pose proof (node_rep_split_sep L Ls Lf L1 L2 head curr pred succ key) 
           as Htemp; auto.
@@ -65,12 +79,9 @@ Module ContainsSpec (Params: LAZY_LIST_PARAMS).
           assert (l = l') as <- by congruence.
 
           wp_load.
-          iMod ("Hclose" with "[Hpt Himp Hown_auth Hown_frac Hown_keys]").
-          {
-            iNext; iExists S, Skeys, L.
-            iPoseProof ("Himp" with "Hpt") as "Hlist".
-            by iFrame.
-          }
+          iPoseProof ("Himp" with "Hpt") as "Hlist".
+          iMod ("Hclose" with "[Hlist Hown_auth Hown_frac Hown_keys]") as "_".
+          { iNext; iExists S, Skeys, L; by iFrame.  }
 
           iModIntro. wp_let. wp_lam. wp_pures.
           case_bool_decide; last lia.
@@ -78,7 +89,8 @@ Module ContainsSpec (Params: LAZY_LIST_PARAMS).
           iModIntro; iFrame.
 
           iPureIntro.
-          rewrite -Hperm; split; intros.
+          rewrite -elem_of_elements Hequiv -Hperm.
+          split; intros.
           * eapply (sorted_node_lt_cover_gap (Ls ++ L1) L2 pred); try lia.
             ++ by rewrite app_ass -Hsplit_join //= app_comm_cons -app_ass -Hcurr app_ass.
             ++ assert (In key (map node_key ([head] ++ L ++ [tail]))) as Hin.
@@ -102,18 +114,59 @@ Module ContainsSpec (Params: LAZY_LIST_PARAMS).
                by rewrite Heq2; left.
             ** inversion Hsplit_join as [[Heq1 Heq2]]; subst.
                by rewrite Heq2 in_app_iff; right; right; left.
-        - rewrite (list_equiv_split curr next ([head] ++ L)); last first.
+        - assert (next ∈ S).
+          {
+            rewrite -elem_of_elements -Hperm.
+            destruct Ls; assert (In next (L ++ [tail])) as Hin.
+            + inversion Hsplit_sep. by left.
+            + apply in_app_iff in Hin.
+              destruct Hin as [|[|[]]]; first by eapply elem_of_list_In.
+              inversion Hsplit_sep. inversion Hcurr.
+              subst; exfalso.
+              rewrite -Hsplit_sep in Hsort.
+              do 2 apply node_rep_sorted_app in Hsort as (_ & Hsort).
+              apply Sorted_StronglySorted in Hsort; last first.
+              { unfold Relations_1.Transitive; apply node_lt_transitive. } 
+              inversion Hsort as [|? ? _ Hall]; subst.
+              apply node_rep_forall_app in Hall.
+              destruct Hall as [_ Hall].
+              inversion Hall as [|? ? Hfalse]; subst.
+              rewrite /node_lt in Hfalse.
+              assert (node_key tail = INT_MAX) by auto.
+              lia.
+            + inversion Hsplit_sep. 
+              by apply in_app_iff; right; right; left.
+            + apply in_app_iff in Hin.
+              destruct Hin as [|[|[]]]; first by eapply elem_of_list_In.
+              inversion Hsplit_sep. inversion Hcurr.
+              subst; exfalso.
+              rewrite -Hsplit_sep in Hsort.
+              do 2 apply node_rep_sorted_app in Hsort as (_ & Hsort).
+              apply Sorted_StronglySorted in Hsort; last first.
+              { unfold Relations_1.Transitive; apply node_lt_transitive. } 
+              inversion Hsort as [|? ? _ Hall]; subst.
+              apply node_rep_forall_app in Hall.
+              destruct Hall as [_ Hall].
+              inversion Hall as [|? ? Hfalse]; subst.
+              rewrite /node_lt in Hfalse.
+              assert (node_key tail = INT_MAX) by auto.
+              lia.
+          }
+
+          iMod (own_update with "Hown_auth") as "[Hown_auth Hown_auth_frag]".
+          { apply auth_update_alloc, (gset_local_update_union _ _ {[ next ]}). }
+          assert (ε ∪ {[ next ]} = {[ next ]}) as -> by set_solver.
+          assert (S ∪ {[ next ]} = S) as -> by set_solver.
+        
+          rewrite (list_equiv_split curr next ([head] ++ L)); last first.
           { simpl in *. by rewrite -Hsplit_sep. }
           iDestruct "Hlist" as (l' γ) "(>%Hsome & Hpt & #Hlock & Himp)".
           assert (l = l') as <- by congruence.
 
           wp_load.
-          iMod ("Hclose" with "[Hpt Himp Hown_auth Hown_frac Hown_keys]").
-          {
-            iNext; iExists S, Skeys, L.
-            iPoseProof ("Himp" with "Hpt") as "Hlist".
-            by iFrame.
-          }
+          iPoseProof ("Himp" with "Hpt") as "Hlist".
+          iMod ("Hclose" with "[Hlist Hown_auth Hown_frac Hown_keys]") as "_".
+          { iNext; iExists S, Skeys, L; by iFrame. }
 
           iModIntro. wp_let. wp_lam. wp_pures.
           case_bool_decide as Hcase.
@@ -150,65 +203,56 @@ Module ContainsSpec (Params: LAZY_LIST_PARAMS).
             eapply node_lt_le_incl, Forall_forall; eauto.
             rewrite elem_of_list_In //=.
           * wp_if.
-            iApply ("IH" $! next with "[Hown_frag] [%] [%]").
-            { iFrame. }
-            { 
-              right. rewrite -elem_of_elements -Hperm.
-              destruct Ls; assert (In next (L ++ [tail])) as Hin.
-              -- inversion Hsplit_sep. by left.
-              -- apply in_app_iff in Hin.
-                 destruct Hin as [|[|[]]]; first by eapply elem_of_list_In.
-                 subst; exfalso. 
-                 rewrite /node_key/tail//= in Hcase; lia.
-              -- inversion Hsplit_sep. 
-                 by apply in_app_iff; right; right; left.
-              -- apply in_app_iff in Hin.
-                 destruct Hin as [|[|[]]]; first by eapply elem_of_list_In.
-                 subst; exfalso. 
-                 rewrite /node_key/tail//= in Hcase; lia.
-            }
+            iApply ("IH" $! next with "[$] [$] [%]").
             { lia. }
 
             iNext; iApply "HΦ".
-      + iInv lazyN as (? ? ?) "(>%Hperm & _ & _ & _ & >Hown_frac & _ & Hlist)" "_".
+      + iInv lazyN as (? ? L) "(>%Hperm & _ & _ & >Hown_auth & >Hown_frac & _ & Hlist)" "_".
         iDestruct (own_valid_2 with "Hown_frac Hown_frag") 
           as %->%frac_auth_agree_L.
 
-        rewrite (list_equiv_invert); last first.
-        { by rewrite -elem_of_list_In Hperm elem_of_elements. }
+        iAssert ((⌜ curr = head ∨ In curr L ⌝)%I) with "[Hown_auth Hown_curr]" as %Hcurr_range.
+        {
+          iDestruct "Hown_curr" as "[Heq|Hown]"; first by iLeft.
+          iDestruct (own_valid_2 with "Hown_auth Hown") 
+            as %[Hvalid%gset_included]%auth_both_valid_discrete.
+          iPureIntro; right. 
+          rewrite -elem_of_list_In Hperm elem_of_elements.
+          set_solver.
+        }
+
+        rewrite (list_equiv_invert); last done.
         iDestruct "Hlist" as (? ? ?) "(_ & >%Hsome & _ & _ & _)".
         congruence.
     Qed.
     
-    Theorem contains_spec (key: Z) (v: val) (Skeys: gset Z) (Γ: lazy_gname)
+    Theorem contains_spec (key: Z) (v: val) (S: gset Z) (Γ: lazy_gname)
       (Hrange: INT_MIN < key < INT_MAX) :
-      {{{ is_lazy_list v Skeys 1 Γ }}}
+      {{{ is_lazy_list v S 1 Γ }}}
         contains v #key
       {{{ (b: bool), RET #b; 
-        is_lazy_list v Skeys 1 Γ
+        is_lazy_list v S 1 Γ
         ∗
-        ⌜ if b then key ∈ Skeys else key ∉ Skeys ⌝
+        ⌜ if b then key ∈ S else key ∉ S ⌝
       }}}.
     Proof.
       iIntros (Φ) "H HΦ".
-      iDestruct "H" as (h head S) "(%Hv & Hpt & %Hmin & %Hequiv & Hown & #Hinv)".
+      iDestruct "H" as (h head) "(%Hv & Hpt & %Hmin & Hown & #Hinv)".
       wp_lam. wp_let. rewrite -Hv. wp_load.
       wp_apply (find_spec with "[Hown]").
-      { iFrame "# ∗". iPureIntro; split. by left. lia. }
+      { iFrame "# ∗". iSplit. by iLeft. iPureIntro; lia. }
       iIntros (pred succ) "(Hown & %Hkey_in_S)".
       wp_let. wp_match. wp_pures. wp_lam. wp_pures.
 
       iModIntro; case_bool_decide.
       + iApply "HΦ". iSplit. 
-        iExists h, head, S. by iFrame "# ∗".
-        iPureIntro. rewrite /key_equiv in Hequiv. 
-        rewrite -elem_of_elements Hequiv Hkey_in_S.
-        congruence.
+        iExists h, head. by iFrame "# ∗".
+        iPureIntro.
+        rewrite Hkey_in_S; congruence.
       + iApply "HΦ". iSplit. 
-        iExists h, head, S. by iFrame "# ∗".
-        iPureIntro. intros Hin. 
-        rewrite -elem_of_elements Hequiv Hkey_in_S in Hin.
-        congruence.
+        iExists h, head. by iFrame "# ∗".
+        iPureIntro; intros Hin. 
+        rewrite Hkey_in_S in Hin; congruence.
     Qed.
 
   End Proofs.
